\documentclass{article}
\usepackage{amssymb}

\begin{document}
\section*{4.1.5} (page 124)

\subsection*{(a) If a and b are consecutive integers, show that 
$a^2+b^2+(ab)^2$ is a perfect square.}

\subsection*{proof)}
Let $b=a+1$ and substituting into the original expression we arrive at:
$$a^2+(a+1)^2+(a^2+a)^2=a^2+a^2+2a+1+a^4+2a^3+a^2$$
$$a^4+2a^3+2a^2+a^2+2a+1=a^4+a^2+1+2a^3+2a^2+2a$$

We recognize that $(x+y+z)^2=x^2+y^2+z^2+2xy+2yz+2xz$ thus,
$$a^4+a^2+1+2a^3+2a^2+2a=(a^2+a+1)^2$$ which is a perfect square.

\subsection*{(b)If $2a$ is the harmonic mean of $b$ and $c$ (\textit{i.e.} $2a=2/(1/b+1/c)$), show that 
the sum of the squares of the three numbers $a$,$b$, and $c$ is the square of a rational number.}

\subsection*{proof)}
We are to prove that $$a^2+b^2+c^2=\frac{p^2}{q^2},p,q\in \mathbb{Z}, q\neq 0$$.
We substitute $2a=\frac{1}{(\frac{1}{b}+\frac{1}{c})}$ into the expression, and we get:
$$a^2+b^2+c^2=(\frac{1}{(\frac{1}{b}+\frac{1}{c})})^2+b^2+c^2$$
$$(\frac{bc}{bc(\frac{1}{b}+\frac{1}{c})})^2+b^2+c^2=(\frac{bc}{c+b})^2+b^2+c^2$$
$$\frac{b^2c^2}{(c+b)^2}+b^2+c^2=\frac{b^2c^2}{(b+c)^2}+\frac{b^2(b+c)^2}{(b+c)^2}+\frac{c^2(b+c)^2}{(b+c)^2}$$
$$\frac{b^2(b+c)^2+b^2c^2+c^2(b+c)^2}{(b+c)^2}=\frac{b^2(b^2+2bc+c^2)+b^2c^2+c^2(b^2++2bc+c^2)}{(b+c)^2}$$
$$\frac{b^4+2b^3c+b^2c^2+b^2c^2+b^2c^2+2bc^3+c^4}{(b+c)^2}=\frac{b^4+c^4+b^2c^2+2b^3c+2bc^3+2b^2c^2}{(b+c)^2}$$

We recognize that $(x+y+z)^2=x^2+y^2+z^2+2xy+2yz+2xz$ thus,
$$\frac{b^4+c^4+b^2c^2+2b^3c+2bc^3+2b^2c^2}{(b+c)^2}=\frac{(b^2+c^2+bc)^2}{(b+c)^2}$$

\subsection*{(c)If $N$ differs from two successive squares between which 
it lies by $x$ and $y$ respectively, prove that $N-xy$ is a square.}

\subsection*{proof)}
Let's assume the two successive squares are $a^2$ and $(a+1)^2$ and $N$ is placed such that:
$$N-a^2=x$$ $$(a+1)^2-N=y$$ and we need to show that $N-xy$ is a square.

$$N-xy=N-(N-a^2)((a+1)^2-N)$$
$$N-(N-a^2)(a^2+2a+1-N)=N-(a^2N+2aN+N-N^2-a^4-2a^3-a^2+a^2N)$$
$$N-(a^2N+2aN+N-N^2-a^4-2a^3-a^2+a^2N)=N-a^2N-2aN-N+N^2+a^4+2a^3+a^2-a^2N$$
$$N^2+a^4+a^2-2a^2N-2aN+2a^3$$
We recognize that $(x+y+z)^2=x^2+y^2+z^2+2xy+2yz+2xz$ thus,
$$N^2+a^4+a^2-2a^2N-2aN+2a^3=(N-a^2-a)^2$$
which is a square.
\end{document}